regex matcher in regex.v fully verified. hard_star was the hard case

regex.v
@@ -8,9 +8,14 @@ Require Import Ascii.
 Ltac inv H := inversion H; subst; clear H.
 
 (* Borrowed these from another paper, actually about regex derivatives *)
-Definition Sigma := ascii.
-Definition Sigma_dec := Ascii.ascii_dec.
-Axiom Sigma_dec_refl : forall(T : Type) (p1 p2 : T) (a : Sigma), p1 = if Sigma_dec a a then p1 else p2.
+Variable Sigma : Type.
+Variable Sigma_dec : forall(a a' : Sigma), {a = a'} + {a <> a'}.
+Theorem Sigma_dec_refl : forall(T : Type) (p1 p2 : T) (a : Sigma), p1 = if Sigma_dec a a then p1 else p2.
+  intros T p1 p2 a.
+  destruct (Sigma_dec a a).
+  - reflexivity.
+  - contradiction.
+Qed.
 Definition String : Type := list Sigma.
 
 (* Didn't bother with Intersection and Complement yet *)
@@ -145,14 +150,15 @@ Proof.
     + simpl. reflexivity.
 Qed.
 
+(* star_concat upto concat_star necessary for hard star case of der_match *)
 Lemma star_concat :
   forall s r',
     exp_match s (Star r')
     -> (exists xss : list (list Sigma),
-           s = concat xss
-           /\ (forall xs,
-                  In xs xss
-                  -> exp_match xs r')).
+          s = concat xss
+          /\ (forall xs,
+                In xs xss
+                -> exp_match xs r')).
 Proof.
   intros s r' hm.
   remember (Star r') as r. generalize dependent r'. 
@@ -163,6 +169,74 @@ Proof.
     exists (s1 :: xss'); split; auto.
     intros xs hi.
     destruct hi as [hh| ht]; subst; auto.
+Qed.
+
+Definition rm_empty (yss : list String) :=
+  filter (fun l => match l with | [] => false | _ => true end) yss.
+
+Lemma rm_empty_mute : forall(yss : list String),
+    concat (rm_empty yss) = concat yss.
+Proof.
+  intros yss. induction yss.
+  - simpl. reflexivity.
+  - simpl. destruct a.
+    + simpl. apply IHyss.
+    + simpl. rewrite IHyss. reflexivity.
+Qed.
+
+Lemma rm_empty_no_empty : forall(ys : String) (yss : list String),
+    In ys (rm_empty yss) -> ys <> [].
+Proof.
+  intros ys yss H. unfold not. intros C. rewrite C in H.
+  unfold rm_empty in H. induction yss.
+  - simpl in H. contradiction.
+  - simpl in H. destruct a.
+    + apply IHyss in H. contradiction.
+    + simpl in H. destruct H.
+      * discriminate.
+      * apply IHyss in H. contradiction.
+Qed.
+
+Lemma filtered_subset : forall(xs : String) (yss : list String),
+    In xs (rm_empty yss) -> In xs yss.
+Proof.
+  intros xs yss. generalize dependent xs. induction yss; intros xs H.
+  - simpl in H. contradiction.
+  - simpl. destruct a.
+    + simpl in H. right. apply IHyss. apply H.
+    + simpl in H. destruct H.
+      * left. apply H.
+      * right. apply IHyss. apply H.
+Qed.
+
+Lemma star_concat_no_empt : forall(s : String) (r' : regex),
+    s <> []
+    -> exp_match s (Star r')
+    -> (exists xss : list (list Sigma),
+          s = concat xss
+          /\ (forall xs,
+                In xs xss
+                -> exp_match xs r' /\ xs <> [])).
+Proof.
+  intros s r' Hempty Hstar. apply star_concat in Hstar.
+  destruct Hstar as (yss & heq & hall).
+  exists(rm_empty yss). split.
+  - rewrite rm_empty_mute. apply heq.
+  - intros xs H. split.
+    + apply hall.  apply filtered_subset in H. apply H.
+    + apply rm_empty_no_empty in H. apply H.
+Qed.
+
+Lemma concat_star : forall(xss : list String) (r : regex),
+    (forall xs : list Sigma, In xs xss -> exp_match xs r) -> exp_match (concat xss) (Star r).
+Proof.
+  intros xss r H. induction xss.
+  - simpl. apply MStar0.
+  - replace (concat (a :: xss)) with (a ++ (concat xss)).
+    + apply MStarApp.
+      * apply H. simpl. left. reflexivity.
+      * apply IHxss. intros xs H1. apply H. simpl. right. apply H1.
+    + simpl. reflexivity.
 Qed.
                      
 Theorem der_matchb : forall(a : Sigma) (s : String) (r : regex),
@@ -204,16 +278,39 @@ Proof.
     - simpl. inv H.
       + apply IHr1 in H2. apply MUnionL. apply H2.
       + apply IHr2 in H1. apply MUnionR. apply H1.
-    - admit.
-      (*
-      simpl. inv H.
-      + destruct s1.
-        * contradiction.
-        * simpl in H0. injection H0. intros Happ Hchar.
-          rewrite <- Happ. rewrite Hchar in H3. apply IHr in H3.
-          apply MApp.
-          -- apply H3.
-          -- apply H4.*)
+      (* hard_star: This case was the hard one *)
+    - apply star_concat_no_empt in H. destruct H as (xss & heq & hall).
+      + assert (H : exists(s1 : String) (yss : list String),
+                   ((a :: s1) :: yss) = xss).
+        {
+          destruct xss.
+          - simpl in heq. discriminate.
+          - simpl in heq. destruct l eqn:E.
+            + apply hall in E.
+              * contradiction.
+              * rewrite E. simpl. left. reflexivity.
+            + exists(l0). exists(xss). simpl in heq.
+              injection heq. intros I1 I2. rewrite I2. reflexivity.
+        }
+        destruct H as [s1]. destruct H as [yss].
+        rewrite <- H in hall.
+        assert (A : In (a :: s1) ((a :: s1) :: yss)).
+        { simpl. left. reflexivity. } 
+        simpl. replace s with (s1 ++ (concat yss)).
+        * apply MApp.
+          -- apply IHr. apply hall in A. destruct A. apply H0.
+          -- rewrite H in hall.
+             assert (A1 : forall xs : list Sigma, In xs xss -> exp_match xs r).
+             { intros xs. intros HA1. apply hall in HA1. destruct HA1. apply H0. }
+             apply concat_star. intros xs H1. apply A1.
+             rewrite <- H. simpl. right. apply H1.
+        * assert (A1 : concat ((a :: s1) :: yss) = concat xss).
+          { rewrite H. reflexivity. }
+          assert (A2 : concat ((a :: s1) :: yss) = a :: (s1 ++ (concat yss))).
+          { simpl. reflexivity. }
+          rewrite <- A1 in heq. rewrite A2 in heq. injection heq.
+          intros I. symmetry. apply I.
+      + unfold not. intros C. discriminate.
   }
   {
     generalize dependent s. induction r; intros s H.
@@ -246,7 +343,7 @@ Proof.
         * apply H4.
       + reflexivity.
   }
-Admitted.
+Qed.
 
 Theorem match_iff_matchb : forall(s : String) (r : regex),
     true = exp_matchb s r <-> exp_match s r.
