lexer.v
@@ -32,6 +32,7 @@ Fixpoint max_pref_fn (s : String) (r : regex) : option String :=
     end
   end.
 
+(* If p is a prefix of s, return the remaining suffix. Otherwise return none *)
 (* Maybe it would be better to build the suffix while also building the prefix? *)
 Fixpoint get_suffix (p : String) (s : String) :=
   match p, s with
@@ -42,11 +43,12 @@ Fixpoint get_suffix (p : String) (s : String) :=
   end.
 
 (* couldn't find this in the list library? *)
-Fixpoint fold {X Y: Type} (f: X->Y->Y) (l: list X) (b: Y)
+(* this is fold_left, fold_right is easier to prove things about *)
+Fixpoint foldl {X Y: Type} (f: X->Y->Y) (l: list X) (b: Y)
                          : Y :=
   match l with
   | nil => b
-  | h :: t => f h (fold f t b)
+  | h :: t => f h (foldl f t b)
   end.
 
 (* 
@@ -66,12 +68,81 @@ Fixpoint fold {X Y: Type} (f: X->Y->Y) (l: list X) (b: Y)
    2. the concatention of all pre is equal to code
    3. If suff = x ++ y, then pre ++ x does not match any of the regular expressions from rules
  *)
-Program Fixpoint lex (rules : list Rule) (code : String) {measure (length code)} : list eToken :=
+
+Fixpoint lex (rules : list Rule) (code : String) : list eToken :=
   match code with
   | [] => []
   | _ =>
     let (* find all the maximal prefixes, associating them with a rule as we go *)
       mprefs := map (fun ru => match ru with (a, re) => ((a, re), max_pref_fn code re) end) rules
+    in
+    let (* of these maximal prefixes, find the longest *)
+      mpref := foldl (fun apref1 apref2 =>
+                       match apref1, apref2 with
+                       | (_, None), (_, _) => apref2
+                       | (_, _), (_, None) => apref1
+                       | (_, Some x), (_, Some y) => if (length y) <? (length x)
+                                                    then apref2 else apref1
+                       end
+                    ) mprefs (([], EmptySet), None)
+    in
+    let (* get the associated suffix -- might be better to build this while building the prefix? *)
+      msuff := match mpref with
+                    | (_, None) => None (* This state suggests malformed code *)
+                    | (_, Some x) => get_suffix x code
+               end
+    in
+    match mpref, msuff with
+    | (_, None), _ => [] (* This state suggests malformed code *)
+    | _, None => [] (* This state suggests malformed code, possibly refactor code so this case doesn't arise -- maybe a good reason to return the prefix and suffix together *)
+    | (ru, Some prefix), Some suffix => (ru, prefix, suffix) :: (lex rules suffix)
+    end
+      
+  end.
+
+(*********************************************
+*
+*
+*   Alternative formulation, more modular.
+*
+*
+*********************************************)
+
+Variable State : Type. (* Right now, just a regex *)
+Variable transition : Sigma -> State -> State. (* the derivative function *)
+Variable accepting : State -> bool. (* the nullable function *)
+Variable init_state : regex -> State.
+(* in eRule, the State would be the initial state of the machine after converting from regex *)
+Definition eRule : Type := String * regex * State.
+Definition eeToken : Type := eRule * String * String.
+Definition eeLexemes : Type := list eeToken.
+
+Fixpoint max_pref_fn' (s : String) (state : State) : option String :=
+  match s with
+  (* in a regex approach, accepting := nullable *)
+  | [] => if accepting state then Some [] else None
+  | a :: s' =>
+    let
+      (* in a regex approach, transition := derivative *)
+      state' := transition a state in
+    let
+      mpxs := max_pref_fn' s' state' in
+    
+    match mpxs with
+    | None => if (accepting state') then Some [a] else None
+    | Some s'' => Some (a :: s'')
+    end
+  end.
+
+Program Fixpoint lex' (rules : list Rule) (code : String) {measure (length code)} : list eeToken :=
+  match code with
+  | [] => []
+  | _ =>
+    let
+      erules := map (fun ru => match ru with (a,re) => (a, re, init_state re) end)
+    in
+    let (* find all the maximal prefixes, associating them with a rule as we go *)
+      mprefs := map (fun eru => match eru with (a, re, fsm) => (eru, max_pref_fn' code fsm) end) rules
     in
     let (* of these maximal prefixes, find the longest *)
       mpref := fold (fun apref1 apref2 =>
@@ -92,7 +163,7 @@ Program Fixpoint lex (rules : list Rule) (code : String) {measure (length code)}
     match mpref, msuff with
     | (_, None), _ => [] (* This state suggests malformed code *)
     | _, None => [] (* This state suggests malformed code *)
-    | (ru, Some prefix), Some suffix => (ru, prefix, suffix) :: (lex rules suffix)
+    | (eru, Some prefix), Some suffix => (eru, prefix, suffix) :: (lex' rules suffix)
     end
       
   end.
